src/Prelude/ListCRM.v
@@ -1,4 +1,4 @@
-Require Import List.
+From Stdlib Require Import List.
 Import ListNotations.
 From Stdlib Require Import Program.Equality.
 
